semantics for merge

EffectSSA/Trace/Compat.lean
@@ -15,17 +15,34 @@ variable {τ} [MemoryModel τ]
 
 namespace Trace
 
+/--
+Compatibility relation on traces, written as `es ⌣ ds`
+
+Two traces are compatible if their events are pairwise compatible according
+to the memory model. Undefined behavior (UB) is not compatible with anything.
+-/
 inductive Compat : Trace τ → Trace τ → Prop
   | seq :
-      (∀ x ∈ xs, ∀ y ∈ ys, MemoryModel.Compat x y)
+      (∀ x ∈ xs, ∀ y ∈ ys, x ⌣ₑ y)
       → Trace.Compat (.seq xs) (.seq ys)
-
--- N.B: Should UB be compatible with everything, or with nothing?
--- I don't think it actually matters, as merging incompatible traces simply
--- yields UB, but if UB was deemed compatible, then appending the other trace
--- to UB still just yields UB. Thus, I'll say that UB is *NOT* compatible with
--- anything, since that's the shorter definition.
-
 infixl:60 " ⌣ " => Compat
+
+/-!
+Compatibility is decidable.
+-/
+section Decide
+
+theorem seq_compat_seq_iff {xs ys : List (Event τ)} :
+    (.seq xs ⌣ .seq ys) ↔ ∀ x ∈ xs, ∀ y ∈ ys, x ⌣ₑ y :=
+  ⟨fun (Compat.seq h) => h, Compat.seq⟩
+
+instance : DecidableRel (@Compat τ _)
+  | .seq _, .seq _ => decidable_of_iff _ seq_compat_seq_iff.symm
+  | .ub, _ | _, .ub => .isFalse (by rintro ⟨⟩)
+
+end Decide
+
+
+
 
 end Trace
